implementing pip state, proof started, successor part finished

developmentCS/Hoare_getFstShadow.v
@@ -21,6 +21,7 @@ Require Import HoareA.
 Require Import THoareA.
 Require Import Lib.
 Require Import Pip_state.
+Import List.ListNotations.
 
 Module Hoare_Test_FstShadow <: IdModType.
 
@@ -45,29 +46,32 @@ Definition getSh1idx : Exp := Val (cst index sh1idx). (** Return in the original
 
 (** ReadPhysical -page -index : reads physical address *)
 
-Definition xf_read (p: page) : XFun index (option value) := {|
-   b_mod := fun s i => match (lookup p i s.(memory) beqPage beqIndex) with
-                            | Some (PP a) => (s,Some (PP a))
-                            | _ => (s,None) 
-                       end  
+Definition readPhysicalInternal p i memory :option page := 
+match (lookup p i memory beqPage beqIndex) with
+                            | Some (PP a) => Some a
+                            | _ => None
+                       end.
+
+Definition xf_read (p: page) : XFun index (option page) := {|
+   b_mod := fun s i => (s,readPhysicalInternal p i (memory s))
 |}.                                  
 
 Instance VT_index : ValTyp index.
-Instance VT_option_value : ValTyp (option value).
+Instance VT_option_page : ValTyp (option page).
 
 Definition ReadPhysical (p:page) (x:Id) : Exp :=
-  Modify index (option value) VT_index VT_option_value (xf_read p) (Var x).  
+  Modify index (option page) VT_index VT_option_page (xf_read p) (Var x).  
 
 (** Succ -index : calculates the successor of an index *)                 
 
-Definition succInternal (idx:index) : option index :=
+Definition succIndexInternal (idx:index) : option index :=
 let (i,P):=idx in 
   if lt_dec i tableSize 
   then Some (CIndex i) 
   else None.
 
 Definition xf_succ : XFun index (option index) := {|
-   b_mod := fun s (idx:index) =>  (s, succInternal idx)
+   b_mod := fun s (idx:index) =>  (s, succIndexInternal idx)
 |}.
 
 Instance VT_option_index : ValTyp (option index).
@@ -83,16 +87,214 @@ Definition getFstShadow (p:page) : Exp :=
                       (ReadPhysical p "y")
            ).
 
+(******* getPartitions from StateLib *)
+
+Fixpoint getAllIndicesAux (pos count: nat) : list index :=
+  match count with
+    | 0        => []
+    | S count1 => match lt_dec pos tableSize with
+                   | left pf => Build_index pos pf :: getAllIndicesAux (S pos) count1
+                   | _       => []
+                 end
+  end.
+
+(** The [getAllIndicesAux] function returns the list of all indices  *)
+Definition getAllIndices := getAllIndicesAux 0 tableSize.
+
+Fixpoint getAllVAddrAux (levels: nat) : list (list index) :=
+  match levels with
+    | 0         => [[]]
+    | S levels1 => let alls := getAllVAddrAux levels1 in
+                  flat_map (fun (idx : index) => map (cons idx) alls) getAllIndices
+  end.
+
+(** The [getAllVAddr] function returns the list of all virtual addresses *)
+Definition getAllVAddr := map CVaddr (getAllVAddrAux (S nbLevel)).
+
+(**  The [getPd] function returns the physical page of the page directory of
+     a given partition  *)
+Definition getPd partition memory: option page:= 
+match succIndexInternal PDidx with 
+|None => None
+|Some idx => readPhysicalInternal partition idx memory
+end. 
+
+
+(** The [getNbLevel] function returns the number of translation levels of the MMU *) 
+Definition getNbLevel : option level:=
+if gt_dec nbLevel 0
+then Some (CLevel (nbLevel-1))
+else None.
+
+(** The [filterOption] function Remove option type from list *)
+Fixpoint filterOption (l : list (option page)) := 
+match l with 
+| [] => []
+| Some a :: l1 => a:: filterOption l1
+|None :: l1 => filterOption l1
+end.
+
+Definition getIndexOfAddr (va : vaddr) (l : level) : index:=
+nth ((length va) - (l + 2))  va (CIndex 0) .
+
+Definition eqbLevel (a b : level) : bool:= a =? b.
+
+Program Definition predLevel (n : level) : option level := 
+if gt_dec n 0 then
+let ipred := n-1 in 
+Some (Build_level ipred _ )
+else  None.
+Next Obligation.
+destruct n.
+simpl.
+omega.
+Qed.
+
+(** The [readPhyEntry] function returns the physical page stored into a given table 
+    at a given position in memory. The table should contain only Physical entries 
+    (The type [PE] is already defined in [Model.ADT]) *)
+Definition readPhyEntry(paddr : page) (idx : index) memory: option page :=
+let entry :=  lookup paddr idx memory beqPage beqIndex  in 
+  match entry with
+  | Some (PE a) => Some a.(pa)
+  | Some _ => None
+  | None => None
+ end. 
+
+(** The [getIndirection] function returns the configuration table entry that corresponds 
+    to the given level and virtual address *)
+Fixpoint  getIndirection (pd : page) (va : vaddr) (currentlevel : level) (stop : nat) s :=
+match stop with 
+|0 => Some pd 
+|S stop1 => 
+if (eqbLevel currentlevel fstLevel)  
+then Some pd 
+  else  
+    let idx :=  getIndexOfAddr va currentlevel in 
+       match readPhyEntry pd idx s.(memory) with 
+       | Some addr =>  if  defaultPage =? addr 
+                          then Some defaultPage 
+                          else 
+                            match predLevel currentlevel with
+                            |Some p =>  getIndirection addr va p stop1 s
+                            |None => None
+                            end
+      |None => None
+    end
+   end. 
+
+(** The [readPresent] function returns the flag value stored into a given table 
+    at a given position in memory. The table should contain only Physical entries 
+    (The type [PE] is already defined in [Model.ADT]) *)
+Definition readPresent  (paddr : page) (idx : index) memory : option bool:=
+let entry :=  lookup paddr idx memory beqPage beqIndex  in 
+  match entry with
+  | Some (PE a) => Some a.(present)
+  | Some _ => None
+  | None => None
+ end. 
+
+(** The [getMappedPage] function returns the physical page stored into a leaf node, 
+   which corresponds to a given virtual address, if the present flag is equal to true **)
+Definition getMappedPage pd s va: option page :=
+match getNbLevel  with 
+ |None => None
+ |Some level => let idxVA := getIndexOfAddr va fstLevel  in 
+               match getIndirection pd va level (nbLevel - 1) s with 
+                | Some tbl =>  if defaultPage =? tbl
+                                   then None 
+                                   else match (readPresent tbl idxVA s.(memory)) with 
+                                         |Some true => readPhyEntry tbl idxVA s.(memory) 
+                                         | _ =>  None 
+                                        end
+                | _ => None
+               end
+end.
+
+
+(** The [getMappedPagesOption] function Return all physical pages marked as 
+    present into a partition *)
+Definition getMappedPagesOption (pd : page) (vaList : list vaddr) s : list (option page) :=
+map (getMappedPage pd s) vaList.
+
+(** The [getMappedPagesAux] function removes option type from mapped pages list *)
+Definition getMappedPagesAux (pd :page)  (vaList : list vaddr) s : list page := 
+filterOption (getMappedPagesOption pd vaList s).
+
+(** The [readPDflag] function returns the flag value stored into a given table 
+    at a given position in memory. The table should contain only virtual entries 
+    (The type [VE] is already defined in [Model.ADT])  *)
+Definition readPDflag  (paddr : page) (idx : index) memory : option bool:=
+let entry :=  lookup paddr idx memory beqPage beqIndex  in 
+  match entry with
+  | Some (VE a) => Some a.(pd)
+  | Some _ => None
+  | None => None
+ end.
+
+(**  The [getFstShadow] returns the physical page of the first shadow page of
+     a given partition  *)
+Definition getFstShadowInternal partition memory: option page:= 
+match succIndexInternal sh1idx with 
+|None => None
+|Some idx => readPhysicalInternal partition idx memory
+end. 
+
+(** The [checkChild] function returns true if the given virtual address corresponds 
+    to a child of the given partition 
+    *)
+Definition checkChild partition level (s:state) va : bool :=
+let idxVA :=  getIndexOfAddr va fstLevel in 
+match getFstShadowInternal partition s.(memory)  with 
+| Some sh1  => 
+   match getIndirection sh1 va level (nbLevel -1) s with 
+    |Some tbl => if tbl =? defaultPage 
+                    then false 
+                    else match readPDflag tbl idxVA s.(memory) with 
+                          |Some true => true
+                          |_ => false
+                          end
+    |None => false 
+    end
+| _ => false
+end.
+
+(** The [getPdsVAddr] function returns the list of virtual addresses used as 
+    partition descriptor into a given partition *)
+Definition getPdsVAddr partition l1 (vaList : list vaddr) s :=
+filter (checkChild partition l1 s) vaList.
+
+
+(** The [getChildren] function Returns all children of a given partition *)
+Definition getChildren (partition : page) s := 
+let vaList := getAllVAddr in 
+match getNbLevel, getPd partition s.(memory) with 
+|Some l1,Some pd => getMappedPagesAux pd (getPdsVAddr partition l1 vaList s) s
+|_, _ => []
+end.
+
+(** The [getPartitionsAux] function returns all pages marked as descriptor partition *)
+Fixpoint getPartitionAux (partitionRoot : page) (s : W) bound {struct bound} : list page :=
+  match bound with
+    | O => []
+    | S bound1 => partitionRoot :: flat_map (fun p => getPartitionAux p s bound1) 
+                                    (getChildren partitionRoot s )
+  end.
+
+(** The [getPartitions] function fixes the sufficient timeout value to retrieve all partitions *)
+Definition getPartitions (root : page) s : list page  :=
+(getPartitionAux root s (nbPage+1)). 
+
+
 (******* State properties *)
 
-(** partitionDescriptorEntry *) 
 Definition isVA (p:page) (i:index) (s:W): Prop := match (lookup p i (s.(memory)) beqPage beqIndex) with 
              |Some (VA _) => True
              |_ => False
              end.
 
 Definition nextEntryIsPP (p:page) (idx:index) (p':Value) (s:W) : Prop:= 
-match succInternal idx with 
+match succIndexInternal idx with 
 | Some i => match lookup p i (memory s) beqPage beqIndex with 
                   | Some (PP table) => p' = cst value (PP table)
                   |_ => False 
@@ -100,15 +302,97 @@ match succInternal idx with
 | _ => False 
 end.
 
-Definition getPartitions (multiplexer:page) (s:W) := @nil page.
-
 Definition partitionDescriptorEntry (s:W) := 
 forall (p : page),  
-In p (getPartitions multiplexer s)-> 
-forall (idx : index), (idx = PDidx \/ idx = sh1idx \/ idx = sh2idx \/ idx = sh3idx \/ idx = PPRidx  \/ idx = PRidx ) ->
-isVA p idx  s /\ 
-exists (p1:page) , nextEntryIsPP p idx (cst value (PP p1)) s  /\  
-(cst page p1) <> (cst page pageinit).
+  In p (getPartitions multiplexer s)-> forall (idx : index), 
+    (idx = PDidx \/ idx = sh1idx \/ idx = sh2idx \/ idx = sh3idx \/ idx = PPRidx  \/ idx = PRidx ) ->
+    idx < tableSize - 1  /\ isVA p idx  s /\ exists (p1:page) , nextEntryIsPP p idx (cst value (PP p1)) s  /\  
+    (cst page p1) <> (cst page defaultPage).
+
+
+(******* Useful Lemmas *)
+
+(** about getSh1idx *)
+
+Lemma getSh1idxW (P: Value -> W -> Prop) (fenv: funEnv) (env: valEnv) :
+  {{wp P fenv env getSh1idx}} fenv >> env >> getSh1idx {{P}}.
+Proof.
+apply wpIsPrecondition.
+Qed.
+
+Lemma getSh1idxWp P fenv env :
+{{fun s => P s }} fenv >> env >> getSh1idx 
+{{fun (idxSh1 : Value) (s : state) => P s  /\ idxSh1 = cst index sh1idx }}.
+Proof.
+eapply weakenEval.
+eapply getSh1idxW.
+intros. 
+unfold wp.
+intros.
+unfold getSh1idx in X2.
+inversion X2;subst.
+auto.
+inversion X3.
+Qed.
+
+(** about Succ *)
+
+Require Import Coq.Logic.Eqdep.
+
+Lemma succW  (x : Id) (P: Value -> W -> Prop) (v:Value) (fenv: funEnv) (env: valEnv) :
+forall (idx:index), {{fun s => idx < (tableSize -1) /\ forall  l : idx + 1 < tableSize , 
+    P (cst (option index) (succIndexInternal idx)) s /\ v = cst index idx }}  fenv >> (x,v)::env >> Succ x {{ P }}.
+Proof.
+intros.
+unfold THoareTriple_Eval.
+intros.
+intuition.
+destruct H1 as [H1 H1'].
+omega.
+inversion X;subst.
+inversion X0;subst.
+repeat apply inj_pair2 in H7;subst.
+inversion X2;subst.
+inversion X3;subst.
+inversion H;subst.
+destruct IdModP.IdEqDec in H3.
+inversion H3;subst.
+clear H3 e X3 H XF1.
+inversion X1;subst.
+inversion X3;subst.
+repeat apply inj_pair2 in H7.
+repeat apply inj_pair2 in H9.
+subst.
+unfold b_exec in *.
+unfold b_eval in *.
+unfold xf_succ in *.
+unfold b_mod in *.
+simpl in *.
+inversion X4;subst.
+apply H1.
+inversion X5.
+inversion X5.
+contradiction.
+Qed.
+
+Lemma succWp (x:Id) (v:Value) P (fenv: funEnv) (env: valEnv) :
+forall (idx:index), {{fun s => P s  /\ idx < tableSize - 1 /\ v=cst index idx}} fenv >> (x,v)::env >> Succ x 
+{{fun (idxsuc : Value) (s : state) => P s  /\ cst (option index) (succIndexInternal idx) = idxsuc }}.
+Proof.
+intros.
+eapply weakenEval.
+eapply succW.
+intros.
+simpl.
+split.
+instantiate (1:=idx).  
+intuition.
+intros.
+split. 
+intuition.
+intuition.
+Qed.
+
 
 (** Hoare Triple *)
 
@@ -116,6 +400,14 @@ Lemma getFstShadow1 (partition : page) (P : W -> Prop) (fenv: funEnv) (env: valE
 {{fun s => P s  /\ partitionDescriptorEntry s /\ In partition (getPartitions multiplexer s)}}
 fenv >> env >> (getFstShadow partition) 
 {{fun (sh1 : Value) (s : state) => P s /\ nextEntryIsPP partition sh1idx sh1 s}}.
+Proof.
+unfold getFstShadow.
+eapply BindS_VHTT1.
+eapply getSh1idxWp.
+intros; simpl.
+eapply BindS_VHTT1.
+eapply weakenEval.
+eapply succW.
 Admitted.
 
 
